Earley_WorkSet.thy
@@ -1,0 +1,42 @@
+theory Earley_WorkSet
+  imports 
+    Earley_Set
+begin
+
+locale Earley_WorkSet = Earley_Set +
+  assumes nonempty_deriv: "N \<in> \<NN> \<Longrightarrow> \<not> derives [N] []"
+begin
+
+definition Complete_W :: "nat \<Rightarrow> items \<Rightarrow> items \<Rightarrow> items" where
+  "Complete_W k W I =
+    { inc_item x k | x y.
+        x \<in> bin I (item_origin y) \<and>
+        y \<in> bin W k \<and>
+        is_complete y \<and>
+        next_symbol x = Some (item_rule_head y) }"
+
+function \<pi>_W :: "nat \<Rightarrow> items \<Rightarrow> items \<times> items \<Rightarrow> items \<times> items" where
+  "\<pi>_W k W (I,J) = (
+    if W = {} then (I,J)
+    else
+      let J' = J \<union> Scan k W in
+      let T = Predict k W \<union> Complete_W k W I in
+      let W' = T - I in
+      let I' = I \<union> T in
+      \<pi>_W k W' (I',J'))"
+  by pat_completeness simp
+termination sorry
+
+fun \<I>_W' :: "nat \<Rightarrow> items \<times> items" where
+  "\<I>_W' 0 = \<pi>_W 0 Init (Init,{})"
+| "\<I>_W' (Suc k) = (
+    let (I,J) = \<I>_W' k in
+    \<pi>_W (Suc k) J (I \<union> J, {}))"
+
+definition \<I>_W :: "nat \<Rightarrow> items" where
+  "\<I>_W k = (let (I,J) = \<I>_W' k in I \<union> J)"
+
+definition \<II>_W :: "items" where
+  "\<II>_W = \<I>_W (length inp)"
+
+end
